viper-total-heaps/TotalFraming.thy
@@ -1,0 +1,101 @@
+section \<open>Framed Assertions\<close>
+
+theory TotalFraming
+  imports TotalInhaleExhale
+begin
+
+
+text \<open>We have two definitions of self-framing at the moment. We need to prove their equivalance eventually.\<close>
+
+
+subsection \<open>Self-Framing Assertion Definition Based on \<^const>\<open>red_inhale\<close>\<close>
+
+definition assertion_framing_state :: "'a total_context \<Rightarrow> ('a full_total_state \<Rightarrow> bool) \<Rightarrow> assertion \<Rightarrow> 'a full_total_state \<Rightarrow> bool"
+  where
+    "assertion_framing_state ctxt StateCons A \<omega> \<equiv> 
+      \<forall> res. red_inhale ctxt StateCons A \<omega> res \<longrightarrow> res \<noteq> RFailure"
+
+definition assertion_self_framing_store :: "'a total_context \<Rightarrow> ('a full_total_state \<Rightarrow> bool) \<Rightarrow> assertion \<Rightarrow> 'a store \<Rightarrow> bool"
+  where
+    "assertion_self_framing_store ctxt StateCons A \<sigma> \<equiv> 
+      \<forall> \<omega>. assertion_framing_state ctxt StateCons A (update_store_total \<omega> \<sigma>)"
+
+lemma assertion_framing_star: 
+  assumes "assertion_framing_state ctxt StateCons (A1 && A2) \<omega>" 
+  shows "assertion_framing_state ctxt StateCons A1 \<omega> \<and> 
+        (\<forall> \<omega>'. red_inhale ctxt StateCons A1 \<omega> (RNormal \<omega>') \<longrightarrow> assertion_framing_state ctxt StateCons A2 \<omega>')" (is "?Goal1 \<and> ?Goal2")
+proof 
+  show "assertion_framing_state ctxt StateCons A1 \<omega>"
+    unfolding assertion_framing_state_def
+  proof (rule allI | rule impI)+
+    fix res
+    assume "red_inhale ctxt StateCons A1 \<omega> res"
+
+    thus "res \<noteq> RFailure"
+      using assms InhStarFailureMagic assertion_framing_state_def
+      by blast
+  qed
+next
+  show ?Goal2
+  proof (rule allI | rule impI)+
+    fix \<omega>' 
+    assume InhA1: "red_inhale ctxt StateCons A1 \<omega> (RNormal \<omega>')"
+    show "assertion_framing_state ctxt StateCons A2 \<omega>'"
+      unfolding assertion_framing_state_def
+      using InhA1 InhStarNormal assertion_framing_state_def assms by blast
+  qed
+qed
+
+lemma assertion_framing_imp: 
+  assumes "assertion_framing_state ctxt StateCons (Imp e A) \<omega>"
+     and "ctxt, Some \<omega> \<turnstile> \<langle>e; \<omega>\<rangle> [\<Down>]\<^sub>t (Val (VBool True))"  
+   shows "assertion_framing_state ctxt StateCons A \<omega>"
+  using assms
+  unfolding assertion_framing_state_def
+  by (auto intro: InhImpTrue)
+
+lemma assertion_framing_cond_assert_true:
+  assumes "assertion_framing_state ctxt StateCons (CondAssert e A B) \<omega>"
+      and "ctxt, Some \<omega> \<turnstile> \<langle>e; \<omega>\<rangle> [\<Down>]\<^sub>t (Val (VBool True))"
+    shows "assertion_framing_state ctxt StateCons A \<omega>"
+  using assms
+  unfolding assertion_framing_state_def
+  by (auto intro: InhCondAssertTrue)
+
+lemma assertion_framing_cond_assert_false:
+  assumes "assertion_framing_state ctxt StateCons (CondAssert e A B) \<omega>"
+      and "ctxt, Some \<omega> \<turnstile> \<langle>e; \<omega>\<rangle> [\<Down>]\<^sub>t (Val (VBool False))"
+    shows "assertion_framing_state ctxt StateCons B \<omega>"
+  using assms
+  unfolding assertion_framing_state_def
+  by (auto intro: InhCondAssertFalse)
+
+
+subsection \<open>Self-Framing Predicate Definition Based on \<^const>\<open>sat\<close>\<close>
+
+definition well_typed_store :: "vtyp list \<Rightarrow> ('a \<Rightarrow> abs_type) \<Rightarrow> 'a store \<Rightarrow> bool"
+  where
+    "well_typed_store tys \<Delta> st \<equiv> \<forall>i. i < length tys \<longrightarrow> (\<exists>v. st i = Some v \<and> get_type \<Delta> v = tys ! i)"
+
+definition pred_self_framing :: "'a total_context \<Rightarrow> predicate_decl => bool"
+  where
+    "pred_self_framing ctxt pred_decl \<equiv>
+       \<forall>pred_body \<omega> \<omega>' mh mp frac. predicate_decl.body pred_decl = Some pred_body \<longrightarrow>
+          get_store_total \<omega> = get_store_total \<omega>' \<longrightarrow>
+          \<comment> \<open>well_typed_store (predicate_decl.args pred_decl) (absval_interp_total ctxt) (get_store_total \<omega>) \<longrightarrow>\<close>
+          \<comment> \<open>Maybe well-typed is redundant? \<^const>\<open>sat\<close> implies well-typed.\<close>
+          (\<forall>l. mh l > 0 \<longrightarrow> get_hh_total_full \<omega> l = get_hh_total_full \<omega>' l) \<longrightarrow>
+          sat ctxt \<omega> mh mp (syntactic_mult frac pred_body) \<longrightarrow> sat ctxt \<omega>' mh mp (syntactic_mult frac pred_body)"
+
+lemma pred_self_framing_subst:
+  assumes "pred_self_framing ctxt pred_decl"
+      and "predicate_decl.body pred_decl = Some pred_body"
+      and "get_store_total \<omega> = get_store_total \<omega>'"
+      and "\<forall>l. mh l > 0 \<longrightarrow> get_hh_total_full \<omega> l = get_hh_total_full \<omega>' l"
+      and "sat ctxt \<omega> mh mp (syntactic_mult p pred_body)"
+    shows "sat ctxt \<omega>' mh mp (syntactic_mult p pred_body)"
+  using assms(1) assms(2) assms(3) assms(4) assms(5) pred_self_framing_def
+  by blast
+
+
+end
